ex 7.8

Chap7ex.thy
@@ -8,6 +8,7 @@ fun assigned :: "com \<Rightarrow> vname set" where
 | "assigned (v;; va) = assigned v \<union> assigned va"
 | "assigned (IF v THEN va ELSE vb) = assigned va \<union> assigned vb"
 | "assigned (WHILE v DO va) = assigned va"
+| "assigned (REPEAT v UNTIL va) = assigned v"
 
 lemma "\<lbrakk> (c, s) \<Rightarrow> t; x \<notin> assigned c \<rbrakk> \<Longrightarrow> s x = t x"
   apply (induct rule: big_step_induct)
@@ -19,13 +20,14 @@ fun skip :: "com \<Rightarrow> bool" where
 | "skip (v;; va) = (skip v \<and> skip va)"
 | "skip (IF v THEN va ELSE vb) = (skip va \<and> skip vb)"
 | "skip (WHILE v DO va) = (\<forall>s. \<not>bval v s)"
-
+| "skip (REPEAT v UNTIL va) = (skip v \<and> (\<forall>s. bval va s))"
 lemma "skip c \<Longrightarrow> c \<sim> SKIP"
   apply (induct c rule: skip.induct)
       apply simp_all
   using assign_simp apply auto
    apply (metis Seq Skip)
-  by (meson Skip big_step.IfFalse big_step.IfTrue)
+   apply (meson Skip big_step.IfFalse big_step.IfTrue)
+  using RepeatTrue Skip by presburger
 
 lemma skip_while_aux: "\<lbrakk> (WHILE b DO c, s) \<Rightarrow> s'; bval b s \<rbrakk> \<Longrightarrow> \<not>bval b s'"
   apply (induct "WHILE b DO c" s s' rule: big_step_induct)
@@ -67,6 +69,7 @@ fun skip' :: "com \<Rightarrow> bool" where
 | "skip' (v;; va) = (skip' v \<and> skip' va)"
 | "skip' (IF v THEN va ELSE vb) = (skip' va \<and> skip' vb)"
 | "skip' (WHILE v DO va) = False"
+| "skip' (REPEAT v UNTIL va) = False"
 
 lemma "skip' c \<Longrightarrow> c \<sim> SKIP"
   apply (induct c rule: skip'.induct)
@@ -74,50 +77,16 @@ lemma "skip' c \<Longrightarrow> c \<sim> SKIP"
   apply (metis Seq Skip imp_det)
   by (metis Chap7_2.IfE big_step.IfFalse big_step.IfTrue)
 
-function (sequential) deskip :: "com \<Rightarrow> com" where
+fun deskip :: "com \<Rightarrow> com" where
 "deskip SKIP = SKIP"
 | "deskip (v ::= a) = v ::= a"
 | "deskip (SKIP;; p) = deskip p"
 | "deskip (p;; SKIP) = deskip p"
 | "deskip (p;; q) = (let (p', q') = (deskip p, deskip q) in
-if (p', q') = (p, q) then p;; q else deskip (p';; q'))"
+if p' = SKIP then q' else if q' = SKIP then p' else p';;q')"
 | "deskip (IF b THEN p ELSE q) = IF b THEN deskip p ELSE deskip q"
 | "deskip (WHILE b DO p) = WHILE b DO deskip p"
-  by pat_completeness auto
-
-lemma deskip_term_aux: "\<lbrakk> deskip_dom p; deskip p \<noteq> p \<rbrakk> \<Longrightarrow> size (deskip p) < size p"
-  apply (induct rule: deskip.pinduct)
-  apply (simp_all add: deskip.psimps)
-  by force+
-
-termination deskip
-  apply (relation "measure size")
-                      apply safe
-                      apply (simp_all add: deskip.psimps)
-                      apply (metis One_nat_def Suc_eq_plus1 com.size(8) deskip_term_aux)
-  using deskip.psimps(24) deskip_term_aux apply fastforce
-  using deskip.psimps(25) deskip_term_aux apply fastforce
-                      apply (metis One_nat_def Suc_eq_plus1 com.size(8) deskip_term_aux)
-                     apply (smt (verit, del_insts) Suc_eq_plus1 add.assoc add.commute add.left_commute add_0 add_strict_mono com.size(8) deskip_term_aux nat_add_left_cancel_less)
-                    apply (smt (verit, del_insts) Suc_eq_plus1 add.assoc add.commute add_0 add_strict_mono com.size(8) deskip_term_aux nat_add_left_cancel_less)
-                   apply (smt (z3) One_nat_def com.size(8) com.size(9) deskip.psimps(24) deskip_term_aux less_imp_of_nat_less of_nat_less_imp_less plus_1_eq_Suc zadd_int_left)
-                  apply (smt (verit, ccfv_threshold) com.inject(3) com.size(8) com.size(9) deskip.psimps(24) deskip_term_aux int_ops(1) less_imp_of_nat_less of_nat_Suc of_nat_add of_nat_less_imp_less)
-                 apply (smt (verit, ccfv_threshold) add.comm_neutral add.left_commute add_less_imp_less_right add_less_mono add_mono_thms_linordered_field(2) com.inject(4) com.size(10) com.size(8) deskip.psimps(25) deskip_term_aux less_SucI plus_1_eq_Suc)
-                apply (metis One_nat_def Suc_eq_plus1 add.assoc add_strict_mono com.inject(4) com.size(10) com.size(8) deskip.psimps(25) deskip_term_aux nat_add_left_cancel_less plus_1_eq_Suc)
-               apply (smt (verit, ccfv_threshold) Suc_eq_plus1 add.commute add.left_commute add_0 assigned.cases com.distinct(11) com.distinct(15) com.distinct(19) com.distinct(5) com.exhaust com.inject(3) com.size(8) com.size(9) deskip.psimps(24) deskip_term_aux nat_add_left_cancel_less)
-              apply (smt (z3) One_nat_def com.inject(3) com.size(8) com.size(9) deskip.psimps(24) deskip_term_aux less_imp_of_nat_less of_nat_less_imp_less plus_1_eq_Suc zadd_int_left)
-             apply (smt (z3) One_nat_def com.size(8) com.size(9) deskip.psimps(24) deskip_term_aux less_imp_of_nat_less of_nat_less_imp_less plus_1_eq_Suc zadd_int_left)
-            apply (smt (verit, ccfv_SIG) add_diff_cancel_right' add_less_mono com.inject(3) com.size(9) deskip.psimps(24) deskip_term_aux less_diff_conv)
-           apply (smt (verit, ccfv_threshold) add.comm_neutral add.left_commute add_le_cancel_left add_less_mono com.inject(3) com.size(9) deskip.psimps(24) deskip_term_aux linorder_not_less plus_1_eq_Suc)
-          apply (smt (verit, ccfv_threshold) add_diff_cancel_right' add_less_mono com.inject(3) com.size(10) com.size(9) deskip.psimps(24) deskip.psimps(25) deskip_term_aux less_diff_conv)
-         apply (smt (verit, ccfv_threshold) One_nat_def Suc_eq_plus1 add.assoc add_mono_thms_linordered_field(3) com.inject(4) com.size(10) com.size(9) deskip.psimps(24) deskip.psimps(25) deskip_term_aux nat_add_left_cancel_less not_less_eq order_less_imp_le plus_1_eq_Suc)
-        apply (metis One_nat_def Suc_eq_plus1 Suc_less_eq com.inject(4) com.size(10) deskip.psimps(25) deskip_term_aux)
-       apply (smt (verit, ccfv_threshold) One_nat_def Suc_eq_plus1 add_Suc_right add_diff_cancel_right' add_strict_mono com.inject(4) com.size(10) com.size(8) deskip.psimps(25) deskip_term_aux le_add2 less_diff_conv2)
-      apply (smt (verit, ccfv_threshold) Suc_eq_plus1 add.assoc add.commute add_0 add_diff_cancel_right' add_strict_mono com.size(10) com.size(8) deskip.psimps(25) deskip_term_aux nat_add_left_cancel_less)
-     apply (smt (z3) com.inject(4) com.size(10) com.size(9) deskip.psimps(24) deskip.psimps(25) deskip_term_aux less_imp_of_nat_less of_nat_less_imp_less zadd_int_left)
-    apply (smt (verit, ccfv_threshold) add.commute add_diff_cancel_right' add_le_cancel_left add_less_mono com.inject(3) com.size(10) com.size(9) deskip.psimps(24) deskip.psimps(25) deskip_term_aux linorder_not_less)
-   apply (smt (verit, del_insts) add_diff_cancel_right' add_less_mono com.inject(4) com.size(10) deskip.psimps(25) deskip_term_aux less_diff_conv)
-  by (smt (verit, del_insts) add_less_imp_less_right add_mono_thms_linordered_field(2) add_mono_thms_linordered_field(5) com.inject(4) com.size(10) deskip.psimps(25) deskip_term_aux)
+| "deskip (REPEAT p UNTIL b) = REPEAT deskip p UNTIL b"
 
 lemma "deskip (SKIP ;; WHILE b DO (x ::= a;; SKIP)) = WHILE b DO x ::= a"
   by simp
@@ -125,15 +94,45 @@ lemma "deskip (SKIP ;; WHILE b DO (x ::= a;; SKIP)) = WHILE b DO x ::= a"
 lemma "deskip ((SKIP;; SKIP);; (SKIP;; SKIP)) = SKIP"
   by simp
 
+lemma sim_rep_cong_aux: "(REPEAT c UNTIL b, s) \<Rightarrow> t \<Longrightarrow> c \<sim> c' \<Longrightarrow> (REPEAT c' UNTIL b, s) \<Rightarrow> t"
+  by (induct "REPEAT c UNTIL b" s t rule: big_step_induct; auto)
+
 lemma "deskip c \<sim> c"
   apply (induction c rule: deskip.induct; clarsimp)
-                      defer 8
-                      defer 11
-                      defer 20
-                      prefer 19
-                      apply (blast+)[14]
-         apply ((meson Chap7_2.SeqE Seq)+)[7]
-  using sim_while_cong by presburger
+                      apply safe
+                      apply (blast+)[9]
+  using assign_simp apply auto[13]
+                      apply (metis Chap7_2.SkipE Seq big_step.Assign)
+                      apply auto[2]
+                      apply ((metis Chap7_2.SkipE Seq Skip)+)[8]
+                      apply auto[2]
+                      apply ((metis Chap7_2.SkipE Seq big_step.IfTrue big_step.IfFalse)+)[4]
+                      apply (blast, blast, force)
+                      apply (metis Chap7_2.SkipE Seq)
+                      apply auto[1]
+                      apply blast
+                      apply auto[1]
+                      apply (metis Chap7_2.SkipE Seq)
+                      apply (blast+)[6]
+  using Skip apply auto[2]
+                      apply (metis Chap7_2.SkipE Seq big_step.IfTrue)
+                      apply (metis Chap7_2.SkipE Seq big_step.IfFalse)
+                      apply auto[2]
+                      apply (blast+)[20]
+  using Seq Skip apply force
+                      apply (metis Chap7_2.SkipE Seq)
+                      apply auto[1]
+  using Seq apply presburger
+                      apply (meson Seq big_step.IfTrue)
+                      apply (meson Seq big_step.IfFalse)
+  using Seq big_step.IfTrue apply presburger
+  using Seq big_step.IfFalse apply presburger
+  using Skip apply auto[7]
+                    apply (metis Chap7_2.SkipE Seq)
+                   apply auto[1]
+  using Seq apply presburger
+                 apply (blast+)[12]
+  using sim_while_cong_aux sim_rep_cong_aux by presburger+
 
 inductive astep :: "aexp * state \<Rightarrow> aexp \<Rightarrow> bool" (infix "\<leadsto>" 50) where
 "(V x, s) \<leadsto> N (s x)"
@@ -214,9 +213,16 @@ fun dewhile :: "com \<Rightarrow> com" where
 | "dewhile (p ;; q) = dewhile p ;; dewhile q"
 | "dewhile (IF b THEN p ELSE q) = IF b THEN (dewhile p) ELSE (dewhile q)"
 | "dewhile (WHILE b DO c) = IF (Not b) THEN SKIP ELSE DO c WHILE b"
+| "dewhile (REPEAT c UNTIL b) = REPEAT dewhile c UNTIL b"
+
+lemma sim_rep_cong_aux: "(REPEAT p UNTIL b, s) \<Rightarrow> t \<Longrightarrow> p \<sim> q \<Longrightarrow> (REPEAT q UNTIL b, s) \<Rightarrow> t"
+  by (induct "REPEAT p UNTIL b" s t rule: big_step_induct; auto)
+
+lemma sim_rep_cong: "p \<sim> q \<Longrightarrow> ((REPEAT p UNTIL b) \<sim> (REPEAT q UNTIL b))"
+  by (metis sim_rep_cong_aux)
 
 lemma "dewhile c \<sim> c"
   apply (induct c)
-  using DoWhile_def Seq Skip big_step.IfFalse big_step.IfTrue by auto
+  using DoWhile_def Seq Skip big_step.IfFalse big_step.IfTrue sim_rep_cong by auto
 
 end
